Launchbury/Terms.thy
@@ -22,7 +22,7 @@ nominal_datatype exp =
 | App exp var
 | LetA as::assn body::exp binds "bn as" in body as
 | Lam x::var body::exp binds x in body  ("Lam [_]. _" [100, 100] 100)
-| Null
+| Bool bool
 | IfThenElse exp exp exp  ("((_)/ ? (_)/ : (_))" [0, 0, 10] 10)
 and assn =
   ANil | ACons var exp assn
@@ -156,8 +156,8 @@ lemma Let_distinct[simp]:
   "Lam [v]. e' \<noteq> Let \<Gamma> e"
   "Let \<Gamma> e \<noteq> Lam [v]. e'"
   "Let \<Gamma> e' \<noteq> App e v"
-  "Null \<noteq> Let \<Gamma> e"
-  "Let \<Gamma> e \<noteq> Null"
+  "Bool b \<noteq> Let \<Gamma> e"
+  "Let \<Gamma> e \<noteq> Bool b"
   "(scrut ? e1 : e2) \<noteq> Let \<Gamma> e"
   "Let \<Gamma> e \<noteq> (scrut ? e1 : e2)"
   unfolding Let_def by simp_all
@@ -195,7 +195,7 @@ lemma exp_strong_exhaust:
   assumes "\<And>exp var. y = App exp var \<Longrightarrow> P"
   assumes "\<And>\<Gamma> exp. atom ` domA \<Gamma> \<sharp>* c \<Longrightarrow> y = Let \<Gamma> exp \<Longrightarrow> P"
   assumes "\<And>var exp. {atom var} \<sharp>* c \<Longrightarrow> y = Lam [var]. exp \<Longrightarrow> P"
-  assumes "(y = Null) \<Longrightarrow> P"
+  assumes "\<And> b. (y = Bool b) \<Longrightarrow> P"
   assumes "\<And> scrut e1 e2. y = (scrut ? e1 : e2) \<Longrightarrow> P"
   shows P
   apply (rule  exp_assn.strong_exhaust(1)[where y = y and c = c])
@@ -211,12 +211,12 @@ text {*
 And finally the induction rules with @{term Let}.
 *}
 
-lemma exp_heap_induct[case_names Var App Let Lam Null IfThenElse Nil Cons]:
+lemma exp_heap_induct[case_names Var App Let Lam Bool IfThenElse Nil Cons]:
   assumes "\<And>b var. P1 (Var var)"
   assumes "\<And>exp var. P1 exp \<Longrightarrow> P1 (App exp var)"
   assumes "\<And>\<Gamma> exp. P2 \<Gamma> \<Longrightarrow> P1 exp \<Longrightarrow> P1 (Let \<Gamma> exp)"
   assumes "\<And>var exp. P1 exp \<Longrightarrow> P1 (Lam [var]. exp)"
-  assumes "P1 Null"
+  assumes "\<And> b. P1 (Bool b)"
   assumes "\<And> scrut e1 e2. P1 scrut \<Longrightarrow> P1 e1 \<Longrightarrow> P1 e2 \<Longrightarrow> P1 (scrut ? e1 : e2)"
   assumes "P2 []"
   assumes "\<And>var exp \<Gamma>. P1 exp \<Longrightarrow> P2 \<Gamma> \<Longrightarrow> P2 ((var, exp)#\<Gamma>)"
@@ -236,12 +236,12 @@ proof-
   thus "P1 e" and "P2 \<Gamma>" unfolding asToHeap_heapToAssn.
 qed
 
-lemma exp_heap_strong_induct[case_names Var App Let Lam Null IfThenElse Nil Cons]:
+lemma exp_heap_strong_induct[case_names Var App Let Lam Bool IfThenElse Nil Cons]:
   assumes "\<And>var c. P1 c (Var var)"
   assumes "\<And>exp var c. (\<And>c. P1 c exp) \<Longrightarrow> P1 c (App exp var)"
   assumes "\<And>\<Gamma> exp c. atom ` domA \<Gamma> \<sharp>* c \<Longrightarrow> (\<And>c. P2 c \<Gamma>) \<Longrightarrow> (\<And>c. P1 c exp) \<Longrightarrow> P1 c (Let \<Gamma> exp)"
   assumes "\<And>var exp c. {atom var} \<sharp>* c \<Longrightarrow> (\<And>c. P1 c exp) \<Longrightarrow> P1 c (Lam [var]. exp)"
-  assumes "\<And> c. P1 c Null"
+  assumes "\<And> b c. P1 c (Bool b)"
   assumes "\<And> scrut e1 e2 c. (\<And> c. P1 c scrut) \<Longrightarrow> (\<And> c. P1 c e1) \<Longrightarrow> (\<And> c. P1 c e2) \<Longrightarrow> P1 c (scrut ? e1 : e2)"
   assumes "\<And>c. P2 c []"
   assumes "\<And>var exp \<Gamma> c. (\<And>c. P1 c exp) \<Longrightarrow> (\<And>c. P2 c \<Gamma>) \<Longrightarrow> P2 c ((var,exp)#\<Gamma>)"
@@ -269,14 +269,14 @@ These rules can be used instead of the original induction rules, which require a
 goal for @{typ assn}.
 *}
 
-lemma exp_induct[case_names Var App Let Lam  Null IfThenElse]:
+lemma exp_induct[case_names Var App Let Lam Bool IfThenElse]:
   assumes "\<And>var. P (Var var)"
   assumes "\<And>exp var. P exp \<Longrightarrow> P (App exp var)"
   assumes "\<And>\<Gamma> exp. (\<And> x. x \<in> domA \<Gamma> \<Longrightarrow>  P (the (map_of \<Gamma> x))) \<Longrightarrow> P exp \<Longrightarrow> P (Let \<Gamma> exp)"
   assumes "\<And>var exp.  P exp \<Longrightarrow> P (Lam [var]. exp)"
-  assumes "P Null"
+  assumes "\<And> b. P (Bool b)"
   assumes "\<And> scrut e1 e2. P scrut \<Longrightarrow> P e1 \<Longrightarrow> P e2 \<Longrightarrow> P (scrut ? e1 : e2)"
-  shows "P  exp"
+  shows "P exp"
   apply (rule exp_heap_induct[of P "\<lambda> \<Gamma>. (\<forall>x \<in> domA \<Gamma>. P (the (map_of \<Gamma> x)))"])
   apply (metis assms(1))
   apply (metis assms(2))
@@ -287,14 +287,14 @@ lemma exp_induct[case_names Var App Let Lam  Null IfThenElse]:
   apply auto
   done
 
-lemma  exp_strong_induct_set[case_names Var App Let Lam Null IfThenElse]:
+lemma  exp_strong_induct_set[case_names Var App Let Lam Bool IfThenElse]:
   assumes "\<And>var c. P c (Var var)"
   assumes "\<And>exp var c. (\<And>c. P c exp) \<Longrightarrow> P c (App exp var)"
   assumes "\<And>\<Gamma> exp c.
     atom ` domA \<Gamma> \<sharp>* c \<Longrightarrow> (\<And>c x e. (x,e) \<in> set \<Gamma> \<Longrightarrow>  P c e) \<Longrightarrow> (\<And>c. P c exp) \<Longrightarrow> P c (Let \<Gamma> exp)"
   assumes "\<And>var exp c. {atom var} \<sharp>* c \<Longrightarrow> (\<And>c. P c exp) \<Longrightarrow> P c (Lam [var]. exp)"
-  assumes "\<And> c. P c Null"
-  assumes "\<And> scrut e1 e2 c. (\<And> c. P c scrut) \<Longrightarrow> (\<And> c. P c e1) \<Longrightarrow> (\<And> c. P c e2) \<Longrightarrow> P c (scrut ? e1 : e2)"
+  assumes "\<And>b c. P c (Bool b)"
+  assumes "\<And>scrut e1 e2 c. (\<And> c. P c scrut) \<Longrightarrow> (\<And> c. P c e1) \<Longrightarrow> (\<And> c. P c e2) \<Longrightarrow> P c (scrut ? e1 : e2)"
   shows "P (c::'a::fs) exp"
   apply (rule exp_heap_strong_induct(1)[of P "\<lambda> c \<Gamma>. (\<forall>(x,e) \<in> set \<Gamma>. P c e)"])
   apply (metis assms(1))
@@ -307,13 +307,13 @@ lemma  exp_strong_induct_set[case_names Var App Let Lam Null IfThenElse]:
   done
 
 
-lemma  exp_strong_induct[case_names Var App Let Lam Null IfThenElse]:
+lemma  exp_strong_induct[case_names Var App Let Lam Bool IfThenElse]:
   assumes "\<And>var c. P c (Var var)"
   assumes "\<And>exp var c. (\<And>c. P c exp) \<Longrightarrow> P c (App exp var)"
   assumes "\<And>\<Gamma> exp c.
     atom ` domA \<Gamma> \<sharp>* c \<Longrightarrow> (\<And>c x. x \<in> domA \<Gamma> \<Longrightarrow>  P c (the (map_of \<Gamma> x))) \<Longrightarrow> (\<And>c. P c exp) \<Longrightarrow> P c (Let \<Gamma> exp)"
   assumes "\<And>var exp c. {atom var} \<sharp>* c \<Longrightarrow> (\<And>c. P c exp) \<Longrightarrow> P c (Lam [var]. exp)"
-  assumes "\<And> c. P c Null"
+  assumes "\<And>b c. P c (Bool b)"
   assumes "\<And> scrut e1 e2 c. (\<And> c. P c scrut) \<Longrightarrow> (\<And> c. P c e1) \<Longrightarrow> (\<And> c. P c e2) \<Longrightarrow> P c (scrut ? e1 : e2)"
   shows "P (c::'a::fs) exp"
   apply (rule exp_heap_strong_induct(1)[of P "\<lambda> c \<Gamma>. (\<forall>x \<in> domA \<Gamma>. P c (the (map_of \<Gamma> x)))"])
@@ -361,8 +361,8 @@ lemma fv_App[simp]: "fv (App e x) = insert x (fv e)"
   unfolding fv_def by (auto simp add: exp_assn.supp supp_at_base)
 lemma fv_Let[simp]: "fv (Let \<Gamma> e) = (fv \<Gamma> \<union> fv e) - domA \<Gamma>"
   unfolding fv_def by (auto simp add: Let_supp exp_assn.supp supp_at_base set_bn_to_atom_domA)
-lemma fv_Null[simp]: "fv Null = {}"
-  unfolding fv_def by (auto simp add: exp_assn.supp)
+lemma fv_Bool[simp]: "fv (Bool b) = {}"
+  unfolding fv_def by (auto simp add: exp_assn.supp pure_supp)
 lemma fv_IfThenElse[simp]: "fv (scrut ? e1 : e2)  = fv scrut \<union> fv e1 \<union> fv e2"
   unfolding fv_def by (auto simp add: exp_assn.supp)
 
@@ -492,7 +492,7 @@ nominal_function isLam :: "exp \<Rightarrow> bool" where
   "isLam (Lam [x]. e) = True" |
   "isLam (App e x) = False" |
   "isLam (Let as e) = False" |
-  "isLam Null = False" |
+  "isLam (Bool b) = False" |
   "isLam (scrut ? e1 : e2) = False"
   unfolding isLam_graph_aux_def eqvt_def
   apply simp
@@ -509,7 +509,7 @@ nominal_function isVal :: "exp \<Rightarrow> bool" where
   "isVal (Lam [x]. e) = True" |
   "isVal (App e x) = False" |
   "isVal (Let as e) = False" |
-  "isVal Null = True" |
+  "isVal (Bool b) = True" |
   "isVal (scrut ? e1 : e2) = False"
   unfolding isVal_graph_aux_def eqvt_def
   apply simp
@@ -520,7 +520,7 @@ nominal_function isVal :: "exp \<Rightarrow> bool" where
 nominal_termination (eqvt) by lexicographic_order
 
 lemma isVal_Lam: "isVal (Lam [x]. e)" by simp
-lemma isVal_Null: "isVal Null" by simp
+lemma isVal_Bool: "isVal (Bool b)" by simp
 
 
 subsubsection {* The notion of thunks *}
@@ -578,13 +578,13 @@ lemma nonrec_eqvt[eqvt]:
   "nonrec \<Gamma> \<Longrightarrow> nonrec (\<pi> \<bullet> \<Gamma>)"
   by (erule nonrecE) (auto simp add: nonrec_def)
 
-lemma exp_induct_rec[case_names Var App Let Let_nonrec Lam Null IfThenElse]:
+lemma exp_induct_rec[case_names Var App Let Let_nonrec Lam Bool IfThenElse]:
   assumes "\<And>var. P (Var var)"
   assumes "\<And>exp var. P exp \<Longrightarrow> P (App exp var)"
   assumes "\<And>\<Gamma> exp. \<not> nonrec \<Gamma> \<Longrightarrow> (\<And> x. x \<in> domA \<Gamma> \<Longrightarrow>  P (the (map_of \<Gamma> x))) \<Longrightarrow> P exp \<Longrightarrow> P (Let \<Gamma> exp)"
   assumes "\<And>x e exp. atom x \<sharp> e \<Longrightarrow> P e \<Longrightarrow> P exp \<Longrightarrow> P (let x be e in exp)"
   assumes "\<And>var exp.  P exp \<Longrightarrow> P (Lam [var]. exp)"
-  assumes "P Null"
+  assumes "\<And>b. P (Bool b)"
   assumes "\<And> scrut e1 e2. P scrut \<Longrightarrow> P e1 \<Longrightarrow> P e2 \<Longrightarrow> P (scrut ? e1 : e2)"
   shows "P exp"
   apply (rule exp_induct[of P])
@@ -600,14 +600,14 @@ lemma exp_induct_rec[case_names Var App Let Let_nonrec Lam Null IfThenElse]:
   apply (metis assms(7))
   done
 
-lemma  exp_strong_induct_rec[case_names Var App Let Let_nonrec Lam Null IfThenElse]:
+lemma  exp_strong_induct_rec[case_names Var App Let Let_nonrec Lam Bool IfThenElse]:
   assumes "\<And>var c. P c (Var var)"
   assumes "\<And>exp var c. (\<And>c. P c exp) \<Longrightarrow> P c (App exp var)"
   assumes "\<And>\<Gamma> exp c.
     atom ` domA \<Gamma> \<sharp>* c \<Longrightarrow> \<not> nonrec \<Gamma> \<Longrightarrow> (\<And>c x. x \<in> domA \<Gamma> \<Longrightarrow>  P c (the (map_of \<Gamma> x))) \<Longrightarrow> (\<And>c. P c exp) \<Longrightarrow> P c (Let \<Gamma> exp)"
   assumes "\<And>x e exp c. {atom x} \<sharp>* c \<Longrightarrow> atom x \<sharp> e \<Longrightarrow> (\<And> c. P c e) \<Longrightarrow> (\<And> c. P c exp) \<Longrightarrow> P c (let x be e in exp)"
   assumes "\<And>var exp c. {atom var} \<sharp>* c \<Longrightarrow> (\<And>c. P c exp) \<Longrightarrow> P c (Lam [var]. exp)"
-  assumes "\<And> c. P c Null"
+  assumes "\<And>b c. P c (Bool b)"
   assumes "\<And> scrut e1 e2 c. (\<And> c. P c scrut) \<Longrightarrow> (\<And> c. P c e1) \<Longrightarrow> (\<And> c. P c e2) \<Longrightarrow> P c (scrut ? e1 : e2)"
   shows "P (c::'a::fs) exp"
   apply (rule exp_strong_induct[of P])
@@ -623,14 +623,14 @@ lemma  exp_strong_induct_rec[case_names Var App Let Let_nonrec Lam Null IfThenEl
   apply (metis assms(7))
   done
 
-lemma  exp_strong_induct_rec_set[case_names Var App Let Let_nonrec Lam Null IfThenElse]:
+lemma  exp_strong_induct_rec_set[case_names Var App Let Let_nonrec Lam Bool IfThenElse]:
   assumes "\<And>var c. P c (Var var)"
   assumes "\<And>exp var c. (\<And>c. P c exp) \<Longrightarrow> P c (App exp var)"
   assumes "\<And>\<Gamma> exp c.
     atom ` domA \<Gamma> \<sharp>* c \<Longrightarrow> \<not> nonrec \<Gamma> \<Longrightarrow> (\<And>c x e. (x,e) \<in> set \<Gamma> \<Longrightarrow>  P c e) \<Longrightarrow> (\<And>c. P c exp) \<Longrightarrow> P c (Let \<Gamma> exp)"
   assumes "\<And>x e exp c. {atom x} \<sharp>* c \<Longrightarrow> atom x \<sharp> e \<Longrightarrow> (\<And> c. P c e) \<Longrightarrow> (\<And> c. P c exp) \<Longrightarrow> P c (let x be e in exp)"
   assumes "\<And>var exp c. {atom var} \<sharp>* c \<Longrightarrow> (\<And>c. P c exp) \<Longrightarrow> P c (Lam [var]. exp)"
-  assumes "\<And> c. P c Null"
+  assumes "\<And>b c. P c (Bool b)"
   assumes "\<And> scrut e1 e2 c. (\<And> c. P c scrut) \<Longrightarrow> (\<And> c. P c e1) \<Longrightarrow> (\<And> c. P c e2) \<Longrightarrow> P c (scrut ? e1 : e2)"
   shows "P (c::'a::fs) exp"
   apply (rule exp_strong_induct_set(1)[of P])
